Busybeaver/Deciders/BackwardsReasoning.lean
@@ -1,0 +1,158 @@
+import Busybeaver.Basic
+import Busybeaver.Reachability
+
+namespace TM.Machine
+
+/--
+Holds when the machine cannot take the transition.
+-/
+def unreachable_trans (M: Machine l s) (lab: Label l) (sym: Symbol s) (A: Config l s) :=
+  ∀ (n: ℕ) (C: Config l s), C.state = lab → C.tape.head = sym → ¬(A -[M]{n}-> C)
+
+/--
+If none of the halting transitions are reachable, then the machine does not halt.
+-/
+theorem halting_trans.all_unreachable {M: Machine l s} (h: ∀T ∈ M.halting_trans, M.unreachable_trans T.1 T.2 default):
+  ¬(M.halts default) :=
+by {
+  intro ⟨n, C, Clast, Creach⟩
+  unfold unreachable_trans at h
+  apply absurd Creach
+  apply h (C.state, C.tape.head)
+  · simp [halting_trans]
+    simp [LastState] at Clast
+    exact Clast
+  · rfl
+  · rfl
+}
+
+/-- Underspecified tape for backward steps -/
+abbrev SymbolicTape s := Turing.Tape (WithTop (Symbol s))
+
+/-- Config for backward steps -/
+structure SymbolicConfig (l s) where
+  state: Label l
+  tape: SymbolicTape s
+deriving DecidableEq, Inhabited
+
+section PrettyPrint
+open Std.Format Lean
+
+private def right_repr [Repr α] [Inhabited α] (l: Turing.ListBlank α) (bound: ℕ): List Format := match bound with
+| 0 => []
+| n + 1 => repr l.head :: (right_repr l.tail n)
+
+private def left_repr [Repr α] [Inhabited α] (l: Turing.ListBlank α) (bound: ℕ): List Format := match bound with
+| 0 => []
+| n + 1 => left_repr l.tail n ++ [repr l.head]
+
+instance: Repr (SymbolicConfig l s) := ⟨λ cfg _ ↦
+  Std.Format.joinSep (left_repr cfg.tape.left 10) " " ++ s!" {cfg.state}>{repr cfg.tape.head} " ++ Std.Format.joinSep (right_repr cfg.tape.right 10) " "⟩
+
+end PrettyPrint
+
+def SymbolicConfig.from_trans (lab: Label l) (sym: Symbol s): SymbolicConfig l s := {
+  state := lab,
+  tape := { head := sym, left := default, right := default }
+}
+
+def sym_step (M: Machine l s) (C: SymbolicConfig l s) (sym: Symbol s) (h: M C.state sym ≠ .halt): SymbolicConfig l s :=
+match hM: M C.state sym with
+| .halt => by contradiction
+| .next sym' dir lab' => { state := lab', tape := (C.tape.write ↑sym').move dir }
+
+
+def sym_eval (M: Machine l s) (C: SymbolicConfig l s): Finset (SymbolicConfig l s) := match C.tape.head with
+| ⊤ =>
+  Finset.univ (α:=Symbol s) |>.filter (λ S ↦ M C.state S ≠ .halt) |>.attach.image
+  λ ⟨S, hS⟩ ↦ sym_step M C S (by {
+    simp at hS
+    exact hS
+  })
+| some sym => match hM : M C.state sym with
+  | .halt => {}
+  | .next sym' dir lab' => {
+    sym_step M C sym (by {
+      rw [hM]
+      simp
+    })
+  }
+
+def symbolic_halting (M: Machine l s): Finset (SymbolicConfig l s) :=
+  M.halting_trans.image λ ⟨lab, sym⟩ ↦ SymbolicConfig.from_trans lab sym
+
+def m1RB (l s): Machine l s := λ lab sym ↦ if lab = 0 ∧ sym = 0 then .next 1 .right 1 else .halt
+
+def sym_eval_bw (M: Machine l s) (C: SymbolicConfig l s) (lab: Label l) (sym: Symbol s): Option
+(SymbolicConfig l s) := match M lab sym with
+| .halt => .none
+| .next _ dir lab' =>
+  if lab' ≠ lab then
+    .none
+  else
+    let bw_moved := C.tape.move dir.other
+    match bw_moved.head with
+    | ⊤ => .some { state := lab, tape := bw_moved.write sym }
+    | some sym'' =>
+      if sym'' = sym then
+        .some { state := lab, tape := bw_moved }
+      else
+        .none
+
+def backward_step (M: Machine l s) (C: SymbolicConfig l s): Finset { S: SymbolicConfig l s // C ∈ M.sym_eval S }:=
+  Finset.univ (α:=Label l × Symbol s)
+    |>.filter (λ ⟨L, S⟩ ↦ ∃ sym' dir, M L S = .next sym' dir C.state ∧ (C.tape.move dir.other).head = sym')
+    |>.attach.image λ ⟨⟨L, S⟩, hS⟩ ↦ match hM: M L S with
+    | .halt => by simp_all
+    | .next sym' dir lab' => by {
+      simp_all
+      use { state := L, tape := (C.tape.move dir.other).write S }
+      obtain ⟨sym'', dir', hDefs, hlink⟩ := hS
+      cases hDefs.1
+      cases hDefs.2.1
+      cases hDefs.2.2
+      simp_all
+      simp [sym_eval]
+      simp [Turing.Tape.write]
+      split
+      · simp_all
+      rename_i heq
+      rw [hM] at heq
+      cases heq
+      simp [sym_step]
+      split
+      · rename_i heq
+        rw [hM] at heq
+        cases heq
+      rename_i heq
+      rw [hM] at heq
+      cases heq
+      obtain ⟨Cs, Ch, Cl, Cr⟩ := C
+      simp_all
+      cases dir <;> {
+        simp [Turing.Tape.move, Turing.Tape.write, Turing.Dir.other]
+        simp [Turing.Tape.move, Turing.Dir.other] at hlink
+        rw [← hlink]
+        exact (Turing.ListBlank.cons_head_tail _).symm
+      }
+    }
+
+lemma backward_step.empty_unreachable {C: SymbolicConfig l s} (h: backward_step M C = ∅) (hCh: C.tape.head = some sym):
+  M.unreachable_trans C.state sym A :=
+by {
+  intro n Cc hCcs hCch htrans
+  simp [backward_step, Finset.filter_eq_empty_iff] at h
+  induction htrans using Machine.Multistep.tail_rec with
+  | refl C => {
+    sorry
+  }
+  | tail A B C' n hBC hAB IH => {
+    sorry
+  }
+}
+
+lemma halting_trans.empty_loops {M: Machine l s} (h: M.halting_trans = ∅): ¬(M.halts default) :=
+by {
+  apply all_unreachable
+  simp [h]
+}
